prove one direction of semantic linking for imp

theories/imp.v
@@ -27,6 +27,8 @@ Definition val_to_bool (v : val) : option bool :=
   | _ => None
   end.
 
+Section expr.
+Local Unset Elimination Schemes.
 Inductive expr : Set :=
 | Var (v : string)
 | Val (v : val)
@@ -34,11 +36,36 @@ Inductive expr : Set :=
 | If (e e1 e2 : expr)
 | LetE (v : string) (e1 e2 : expr)
 | Call (f : string) (args : list expr)
+| UbE
 (* Returning to the context, insert automatically during execution. *)
-| ReturnExt (e : expr)
-| Waiting
+| ReturnExt (can_return_further : bool) (e : expr)
+| Waiting (can_return : bool)
 .
+End expr.
+Lemma expr_ind (P : expr → Prop) :
+  (∀ (x : string), P (Var x)) →
+  (∀ (v : val), P (Val v)) →
+  (∀ (e1 : expr) (op : binop) (e2 : expr), P e1 → P e2 → P (BinOp e1 op e2)) →
+  (∀ (e1 e2 e3 : expr), P e1 → P e2 → P e3 → P (If e1 e2 e3)) →
+  (∀ (v : string) (e1 e2 : expr), P e1 → P e2 → P (LetE v e1 e2)) →
+  (∀ (f : string) (args : list expr), Forall P args → P (Call f args)) →
+  (P UbE) →
+  (∀ (can_return_further : bool) (e : expr), P e → P (ReturnExt can_return_further e)) →
+  (∀ (can_return : bool), P (Waiting can_return)) →
+  ∀ (e : expr), P e.
+Proof.
+  move => *. generalize dependent P => P. match goal with | e : expr |- _ => revert e end.
+  fix FIX 1. move => [ ^e] => ????? Hcall ???.
+  6: { apply Hcall. apply Forall_true => ?. by apply: FIX. }
+  all: auto.
+Qed.
 Coercion Val : val >-> expr.
+
+Definition to_val (e : expr) : option val :=
+  match e with
+  | Val v => Some v
+  | _ => None
+  end.
 
 Fixpoint subst (x : string) (v : val) (e : expr) : expr :=
   match e with
@@ -48,8 +75,9 @@ Fixpoint subst (x : string) (v : val) (e : expr) : expr :=
   | If e e1 e2 => If (subst x v e) (subst x v e1) (subst x v e2)
   | LetE y e1 e2 => LetE y (subst x v e1) (if bool_decide (x ≠ y) then subst x v e2 else e2)
   | Call f args => Call f (subst x v <$> args)
-  | ReturnExt e => ReturnExt (subst x v e)
-  | Waiting => Waiting
+  | UbE => UbE
+  | ReturnExt b e => ReturnExt b (subst x v e)
+  | Waiting b => Waiting b
   end.
 Fixpoint subst_l (xs : list string) (vs : list val) (e : expr) : expr :=
   match xs, vs with
@@ -63,6 +91,7 @@ Inductive expr_ectx :=
 | IfCtx (e2 e3 : expr)
 | LetECtx (v : string) (e2 : expr)
 | CallCtx (f : string) (vl : list val) (el : list expr)
+| ReturnExtCtx (can_return_further : bool)
 .
 
 Definition expr_fill_item (Ki : expr_ectx) (e : expr) : expr :=
@@ -72,14 +101,100 @@ Definition expr_fill_item (Ki : expr_ectx) (e : expr) : expr :=
   | IfCtx e2 e3 => If e e2 e3
   | LetECtx v e2 => LetE v e e2
   | CallCtx f vl el => Call f ((Val <$> vl) ++ e :: el)
+  | ReturnExtCtx b => ReturnExt b e
   end.
+
+Global Instance expr_fill_item_inj Ki : Inj (=) (=) (expr_fill_item Ki).
+Proof. destruct Ki => ??? //=; by simplify_eq/=. Qed.
+
+Lemma list_expr_val_eq_inv vl1 vl2 e1 e2 el1 el2 :
+  to_val e1 = None → to_val e2 = None →
+  (Val <$> vl1) ++ e1 :: el1 = (Val <$> vl2) ++ e2 :: el2 →
+  vl1 = vl2 ∧ e1 = e2 ∧ el1 = el2.
+Proof.
+  revert vl2; induction vl1; destruct vl2; intros H1 H2; inversion 1.
+  - done.
+  - subst. by inversion H1.
+  - subst. by inversion H2.
+  - destruct (IHvl1 vl2); auto. split; f_equal; auto.
+Qed.
+
+Lemma list_expr_val_inv vl1 vl2 e2 el2 :
+  (Val <$> vl1) = (Val <$> vl2) ++ e2 :: el2 →
+  is_Some (to_val e2).
+Proof. revert vl2; induction vl1; destruct vl2 => //?; simplify_eq/=; naive_solver. Qed.
+
+Lemma fill_item_val Ki e : is_Some (to_val (expr_fill_item Ki e)) → is_Some (to_val e).
+Proof. destruct Ki => //=; move => [??] //. Qed.
+
+Lemma expr_fill_item_no_val_inj Ki1 Ki2 e1 e2 :
+  to_val e1 = None → to_val e2 = None →
+  expr_fill_item Ki1 e1 = expr_fill_item Ki2 e2 → Ki1 = Ki2.
+Proof.
+  destruct Ki1, Ki2 => //= *; simplify_eq => //.
+  efeed pose proof list_expr_val_eq_inv; [| |done|]; naive_solver.
+Qed.
 
 Definition expr_fill (K : list expr_ectx) (e : expr) : expr :=
   foldl (flip expr_fill_item) e K.
 
+Lemma expr_fill_app K1 K2 e:
+  expr_fill (K2 ++ K1) e = expr_fill K1 (expr_fill K2 e).
+Proof. apply foldl_app. Qed.
+
+Lemma fill_val K e : is_Some (to_val (expr_fill K e)) → is_Some (to_val e).
+Proof.
+  elim/rev_ind: K e => //?? IH e. rewrite expr_fill_app /= => ?.
+  apply IH. by apply: fill_item_val.
+Qed.
+
+Fixpoint static_expr (e : expr) : bool :=
+  match e with
+  | Var v => true
+  | Val v => true
+  | BinOp e1 o e2 => static_expr e1 && static_expr e2
+  | If e e1 e2 => static_expr e && static_expr e1 && static_expr e2
+  | LetE v e1 e2 => static_expr e1 && static_expr e2
+  | Call f args => forallb static_expr args
+  | UbE => true
+  | ReturnExt can_return_further e => false
+  | Waiting can_return => false
+  end.
+
+Lemma static_expr_subst x v e:
+  static_expr e →
+  static_expr (subst x v e).
+Proof.
+  elim: e => //= *; try naive_solver.
+  - by case_bool_decide.
+  - case_bool_decide; naive_solver.
+  - apply forallb_True, Forall_forall => ? /elem_of_list_fmap[?[??]]. subst.
+    revert select (Forall _ _) => /Forall_forall.
+    revert select (Is_true (forallb _ _)) => /forallb_True/Forall_forall. naive_solver.
+Qed.
+
+Lemma static_expr_subst_l xs vs e:
+  static_expr e →
+  length xs = length vs →
+  static_expr (subst_l xs vs e).
+Proof.
+  elim: xs vs e. { by case. }
+  move => ?? IH [//|??] /=???. apply IH; [|lia].
+  by apply static_expr_subst.
+Qed.
+
+Lemma static_expr_expr_fill K e:
+  static_expr (expr_fill K e) ↔ static_expr (expr_fill K (Var "")) ∧ static_expr e.
+Proof.
+  elim/rev_ind: K e => /=. { naive_solver. }
+  move => Ki K IH e. rewrite !expr_fill_app/=.
+  destruct Ki => //=; rewrite ?forallb_app/=; naive_solver.
+Qed.
+
 Record fndef : Type := {
   fd_args : list string;
   fd_body : expr;
+  fd_static : static_expr fd_body;
 }.
 
 Record imp_state := Imp {
@@ -88,8 +203,8 @@ Record imp_state := Imp {
 }.
 Add Printing Constructor imp_state.
 
-Definition initial_imp_state (fns : gmap string fndef) :=
-  Imp Waiting fns.
+Definition initial_imp_state (fns : gmap string fndef) : imp_state :=
+  Imp (Waiting false) fns.
 
 Inductive imp_event : Type :=
 | EICall (fn : string) (args: list val) | EIReturn (ret: val)
@@ -114,6 +229,8 @@ Inductive head_step : imp_state → option imp_event → (imp_state → Prop) �
        ∃ b, val_to_bool v = Some b ∧ σ = Imp (if b then e1 else e2) fns)
 | LetS x v e fns:
   head_step (Imp (LetE x (Val v) e) fns) None (λ σ, σ = Imp (subst x v e) fns)
+| UbES fns:
+  head_step (Imp UbE fns) None (λ σ, False)
 | CallInternalS f fn fns vs:
   fns !! f = Some fn →
   head_step (Imp (Call f (Val <$> vs)) fns) None (λ σ,
@@ -121,17 +238,75 @@ Inductive head_step : imp_state → option imp_event → (imp_state → Prop) �
    σ = Imp (subst_l fn.(fd_args) vs fn.(fd_body)) fns)
 | CallExternalS f fns vs:
   fns !! f = None →
-  head_step (Imp (Call f (Val <$> vs)) fns) (Some (EICall f vs)) (λ σ, σ = Imp Waiting fns)
-| ReturnS fns v:
-  head_step (Imp (ReturnExt (Val v)) fns) (Some (EIReturn v)) (λ σ, σ = (Imp Waiting fns))
-| RecvCallS fns f fn vs:
+  head_step (Imp (Call f (Val <$> vs)) fns) (Some (EICall f vs)) (λ σ, σ = Imp (Waiting true) fns)
+| ReturnS fns v b:
+  head_step (Imp (ReturnExt b (Val v)) fns) (Some (EIReturn v)) (λ σ, σ = (Imp (Waiting b) fns))
+| RecvCallS fns f fn vs b:
   fns !! f = Some fn →
-  length vs = length fn.(fd_args) →
-  head_step (Imp Waiting fns) (Some (EIRecvCall f vs)) (λ σ,
-    σ = (Imp (ReturnExt (subst_l fn.(fd_args) vs fn.(fd_body))) fns))
+  head_step (Imp (Waiting b) fns) (Some (EIRecvCall f vs)) (λ σ,
+    σ = (Imp (if bool_decide (length vs = length fn.(fd_args)) then
+                ReturnExt b (subst_l fn.(fd_args) vs fn.(fd_body))
+              else
+                UbE) fns))
 | RecvReturnS fns v:
-  head_step (Imp Waiting fns) (Some (EIRecvReturn v)) (λ σ, σ = (Imp (Val v) fns))
+  head_step (Imp (Waiting true) fns) (Some (EIRecvReturn v)) (λ σ, σ = (Imp (Val v) fns))
 .
+
+Definition sub_redexes_are_values (e : expr) :=
+  ∀ K e', e = expr_fill K e' → to_val e' = None → K = [].
+
+Lemma sub_redexes_are_values_item e :
+  (∀ Ki e', e = expr_fill_item Ki e' → is_Some (to_val e')) →
+  sub_redexes_are_values e.
+Proof.
+  move => Hitem. elim/rev_ind => //= ?? IH?.
+  rewrite expr_fill_app /= => /Hitem/fill_val[??].
+  naive_solver.
+Qed.
+
+Ltac solve_sub_redexes_are_values := apply sub_redexes_are_values_item; case; naive_solver.
+
+Global Instance expr_fill_inj K : Inj (=) (=) (expr_fill K).
+Proof. induction K as [|Ki K IH]; rewrite /Inj; naive_solver. Qed.
+
+Lemma val_head_stuck e1 σ1 κ Pσ : head_step (Imp e1 σ1) κ Pσ → to_val e1 = None.
+Proof. by inversion 1. Qed.
+
+Lemma head_ctx_step_val Ki e σ1 κ Pσ :
+  head_step (Imp (expr_fill_item Ki e) σ1) κ Pσ → is_Some (to_val e).
+Proof. destruct Ki; inversion 1; simplify_eq => //; by apply: list_expr_val_inv. Qed.
+
+Lemma head_fill_step_val K e σ1 κ Pσ :
+  to_val e = None →
+  head_step (Imp (expr_fill K e) σ1) κ Pσ →
+  K = [].
+Proof.
+  elim/rev_ind: K => //=????. rewrite expr_fill_app /= => /head_ctx_step_val /fill_val[??].
+  naive_solver.
+Qed.
+
+Lemma step_by_val K K' e1' e1_redex σ1 κ Pσ :
+  expr_fill K e1' = expr_fill K' e1_redex →
+  to_val e1' = None →
+  head_step (Imp e1_redex σ1) κ Pσ →
+  ∃ K'', K' = K'' ++ K.
+Proof.
+  assert (fill_val : ∀ K e, is_Some (to_val (expr_fill K e)) → is_Some (to_val e)).
+  { intros K''. induction K'' as [|Ki K'' IH]=> e //=. by intros ?%IH%fill_item_val. }
+  assert (fill_not_val : ∀ K e, to_val e = None → to_val (expr_fill K e) = None).
+  { intros ? e. rewrite !eq_None_not_Some. eauto. }
+
+  intros Hfill Hred Hstep; revert K' Hfill.
+  induction K as [|Ki K IH] using rev_ind=> /= K' Hfill; eauto using app_nil_r.
+  destruct K' as [|Ki' K' _] using @rev_ind; simplify_eq/=.
+  { rewrite expr_fill_app in Hstep. apply head_ctx_step_val in Hstep.
+    apply fill_val in Hstep. by apply not_eq_None_Some in Hstep. }
+  rewrite !expr_fill_app /= in Hfill.
+  assert (Ki = Ki') as ->.
+  { eapply expr_fill_item_no_val_inj, Hfill; eauto using val_head_stuck. }
+  simplify_eq. destruct (IH K') as [K'' ->]; auto.
+  exists K''. by rewrite assoc.
+Qed.
 
 Inductive prim_step : imp_state → option imp_event → (imp_state → Prop) → Prop :=
   Ectx_step K e e' fns κ Pσ:
@@ -139,10 +314,103 @@ Inductive prim_step : imp_state → option imp_event → (imp_state → Prop) �
     head_step (Imp e' fns) κ Pσ →
     prim_step (Imp e fns) κ (λ σ, ∃ e2 fns2, Pσ (Imp e2 fns2) ∧ σ = Imp (expr_fill K e2) fns2).
 
+Lemma prim_step_inv K e fns κ Pσ:
+  prim_step (Imp (expr_fill K e) fns) κ Pσ →
+  to_val e = None →
+  ∃ K' e' Pσ', e = expr_fill K' e' ∧ head_step (Imp e' fns) κ Pσ' ∧
+      Pσ = (λ σ, ∃ e2 fns2, Pσ' (Imp e2 fns2) ∧ σ = Imp (expr_fill (K' ++ K) e2) fns2).
+Proof.
+  inversion 1; simplify_eq => ?.
+  revert select (expr_fill _ _ = expr_fill _ _) => Heq. move: (Heq) => /step_by_val Hg.
+  have [//|? ?]:= Hg _ _ _ _ ltac:(done). subst.
+  rewrite expr_fill_app in Heq. naive_solver.
+Qed.
+
+Lemma prim_step_inv_head K e fns κ Pσ:
+  prim_step (Imp (expr_fill K e) fns) κ Pσ →
+  sub_redexes_are_values e →
+  to_val e = None →
+  ∃ Pσ', head_step (Imp e fns) κ Pσ' ∧
+      Pσ = (λ σ, ∃ e2 fns2, Pσ' (Imp e2 fns2) ∧ σ = Imp (expr_fill K e2) fns2).
+Proof.
+  move => Hprim Hsub ?.
+  move: Hprim => /prim_step_inv[|?[?[?[?[Hstep ?]]]]]. { done. } subst.
+  have ->:= Hsub _ _ ltac:(done). { by apply: val_head_stuck. }
+  naive_solver.
+Qed.
+
 Definition imp_module := Mod prim_step.
+Global Hint Transparent imp_module : tstep.
 
 Global Instance imp_vis_no_all: VisNoAll imp_module.
 Proof. move => *. invert_all' @m_step; invert_all head_step; naive_solver. Qed.
+
+(** * tstep *)
+Lemma imp_step_UbE_s fns K:
+  TStepS imp_module (Imp (expr_fill K UbE) fns) (λ G, G None (λ G', True)).
+Proof.
+  constructor => ? HG. eexists _, _. split; [done|] => /= ??.
+  apply: steps_spec_step_end; [econs; [done|by econs]|] => ? /=?. naive_solver.
+Qed.
+Global Hint Resolve imp_step_UbE_s : tstep.
+
+Lemma imp_step_Waiting_i fns K b:
+  TStepI imp_module (Imp (expr_fill K (Waiting b)) fns) (λ G,
+    (∀ f fn vs, fns !! f = Some fn →
+      G true (Some (EIRecvCall f vs)) (λ G',  G'
+          (Imp (expr_fill K (
+           if bool_decide (length vs = length (fd_args fn)) then
+             ReturnExt b ((subst_l fn.(fd_args) vs fn.(fd_body)))
+           else
+             UbE)) fns))) ∧
+    ∀ v, b → G true (Some (EIRecvReturn v)) (λ G', G' (Imp (expr_fill K v) fns))
+   ).
+Proof.
+  constructor => ? HG. apply steps_impl_step_end => ?? /prim_step_inv_head[| |?[??]].
+  { solve_sub_redexes_are_values. } { done. } subst.
+  invert_all head_step.
+  - naive_solver.
+  - naive_solver.
+Qed.
+Global Hint Resolve imp_step_Waiting_i : tstep.
+
+Lemma imp_step_Waiting_s fns K b:
+  TStepS imp_module (Imp (expr_fill K (Waiting b)) fns) (λ G,
+    (∃ f fn vs, fns !! f = Some fn ∧
+      G (Some (EIRecvCall f vs)) (λ G', G'
+          (Imp (expr_fill K (if bool_decide (length vs = length (fd_args fn)) then
+                               ReturnExt b ((subst_l fn.(fd_args) vs fn.(fd_body)))
+                             else
+                               UbE)) fns))) ∨
+    ∃ v, b ∧ G (Some (EIRecvReturn v)) (λ G', G' (Imp (expr_fill K v) fns))
+   ).
+Proof.
+  constructor => ? HG. destruct_all!; (split!; [done|]) => /= ??. 2: destruct b => //.
+  all: apply: steps_spec_step_end; [econs; [done|by econs]|] => ? /=?; destruct_all?; simplify_eq; done.
+Qed.
+Global Hint Resolve imp_step_Waiting_s : tstep.
+
+Lemma imp_step_ReturnExt_i fns K b (v : val):
+  TStepI imp_module (Imp (expr_fill K (ReturnExt b v)) fns) (λ G,
+    (G true (Some (EIReturn v)) (λ G', G' (Imp (expr_fill K (Waiting b)) fns)))).
+Proof.
+  constructor => ? HG. apply steps_impl_step_end => ?? /prim_step_inv_head[| |?[??]].
+  { solve_sub_redexes_are_values. } { done. } subst.
+  invert_all head_step.
+  naive_solver.
+Qed.
+Global Hint Resolve imp_step_ReturnExt_i : tstep.
+
+Lemma imp_step_ReturnExt_s fns K b (v : val):
+  TStepS imp_module (Imp (expr_fill K (ReturnExt b v)) fns) (λ G,
+    (G (Some (EIReturn v)) (λ G', G' (Imp (expr_fill K (Waiting b)) fns)))).
+Proof.
+  constructor => ? HG. split!; [done|]. move => /= ??.
+  apply: steps_spec_step_end; [econs; [done|by econs]|] => ? /=?.
+  destruct_all?; simplify_eq. done.
+Qed.
+Global Hint Resolve imp_step_ReturnExt_s : tstep.
+
 
 (** * syntactic linking *)
 Definition imp_link (fns1 fns2 : gmap string fndef) : gmap string fndef :=
@@ -246,6 +514,60 @@ Definition imp_prod (fns1 fns2 : gset string) (m1 m2 : module imp_event) : modul
   mod_map (mod_seq_product m1 m2) (imp_prod_filter fns1 fns2).
 Global Hint Transparent imp_prod : tstep.
 
+Inductive imp_link_prod_combine_ectx :
+  nat → bool → bool → imp_prod_filter_state → list expr_ectx → list expr_ectx → list expr_ectx → Prop :=
+| IPCENil:
+  imp_link_prod_combine_ectx 0 false false (IPFState IPFNone []) [] [] []
+| IPCENoneToLeft n cs K Kl Kr bl br:
+  imp_link_prod_combine_ectx n bl br (IPFState IPFNone cs) K Kl Kr →
+  imp_link_prod_combine_ectx (S n) bl br (IPFState IPFLeft (IPFNone :: cs))
+                             (ReturnExtCtx (bl || br)::K) (ReturnExtCtx bl::Kl) Kr
+| IPCENoneToRight n cs K Kl Kr bl br:
+  imp_link_prod_combine_ectx n bl br (IPFState IPFNone cs) K Kl Kr →
+  imp_link_prod_combine_ectx (S n) bl br (IPFState IPFRight (IPFNone :: cs))
+                             (ReturnExtCtx (bl || br)::K) Kl (ReturnExtCtx br::Kr)
+| IPCELeftToRight n cs K Kl Kl' Kr bl br:
+  imp_link_prod_combine_ectx n bl br (IPFState IPFLeft cs) K Kl Kr →
+  static_expr (expr_fill Kl' (Var "")) →
+  imp_link_prod_combine_ectx (S n) true br (IPFState IPFRight (IPFLeft :: cs))
+                             (Kl' ++ K) (Kl' ++ Kl) (ReturnExtCtx br::Kr)
+| IPCELeftToNone n cs K Kl Kl' Kr bl br:
+  imp_link_prod_combine_ectx n bl br (IPFState IPFLeft cs) K Kl Kr →
+  static_expr (expr_fill Kl' (Var "")) →
+  imp_link_prod_combine_ectx (S n) true br (IPFState IPFNone (IPFLeft :: cs))
+                             (Kl' ++ K) (Kl' ++ Kl) Kr
+| IPCERightToLeft n cs K Kl Kr' Kr bl br:
+  imp_link_prod_combine_ectx n bl br (IPFState IPFRight cs) K Kl Kr →
+  static_expr (expr_fill Kr' (Var "")) →
+  imp_link_prod_combine_ectx (S n) bl true (IPFState IPFLeft (IPFRight :: cs))
+                             (Kr' ++ K) (ReturnExtCtx bl::Kl) (Kr' ++ Kr)
+| IPCERightToNone n cs K Kl Kr' Kr bl br:
+  imp_link_prod_combine_ectx n bl br (IPFState IPFRight cs) K Kl Kr →
+  static_expr (expr_fill Kr' (Var "")) →
+  imp_link_prod_combine_ectx (S n) bl true (IPFState IPFNone (IPFRight :: cs))
+                             (Kr' ++ K) Kl (Kr' ++ Kr)
+.
+
+Definition imp_link_prod_inv (bv : bool) (fns1 fns2 : gmap string fndef) (σ1 : imp_module.(m_state)) (σ2 : ((seq_product_state * imp_state * imp_state) * imp_prod_filter_state)) : Prop :=
+  let 'Imp e1 fns1' := σ1 in
+  let '((σsp, Imp el fnsl, Imp er fnsr), σf) := σ2 in
+  ∃ n K Kl Kr e1' el' er' bl br,
+  fns1' = fns1 ∪ fns2 ∧
+  fnsl = fns1 ∧
+  fnsr = fns2 ∧
+  imp_link_prod_combine_ectx n bl br σf K Kl Kr ∧
+  e1 = expr_fill K e1' ∧
+  el = expr_fill Kl el' ∧
+  er = expr_fill Kr er' ∧
+  match σf.(ipf_cur) with
+  | IPFLeft => σsp = SPLeft ∧ e1' = el' ∧ static_expr el' ∧ er' = Waiting br
+              ∧ (if bv then to_val el' = None else True)
+  | IPFRight => σsp = SPRight ∧ e1' = er' ∧ static_expr er' ∧ el' = Waiting bl
+               ∧ (if bv then to_val er' = None else True)
+  | IPFNone => σsp = SPNone ∧ e1' = Waiting (bl || br) ∧ el' = Waiting bl ∧ er' = Waiting br
+  | _ => False
+  end.
+
 Lemma imp_link_refines_prod fns1 fns2:
   fns1 ##ₘ fns2 →
   trefines (MS imp_module (initial_imp_state (imp_link fns1 fns2)))
@@ -254,7 +576,139 @@ Lemma imp_link_refines_prod fns1 fns2:
 Proof.
   move => Hdisj.
   apply tsim_implies_trefines => /= n.
-Admitted.
+  unshelve apply: tsim_remember. { exact: (λ _, imp_link_prod_inv true fns1 fns2). }
+  { split!. 1: by econs. all: done. } { done. }
+  move => /= {}n Hloop [e1 fns1'] [[[? [el fnsl]] [er fnsr] [ipfs cs]]] [K [Kl [Kr ?]]].
+  have {}Hloop : ∀ σi σs,
+            imp_link_prod_inv false fns1 fns2 σi σs
+            → σi ⪯{imp_module, imp_prod (dom (gset string) fns1) (dom (gset string) fns2) imp_module imp_module, n, true} σs. {
+    clear -Hloop. move => [e1 fns1'] [[[sp [el fnsl]] [er fnsr] [ipfs cs]]].
+    move => [m [K [Kl [Kr [e1' [el' [er' [bl [br [?[?[?[HK[?[?[? Hm]]]]]]]]]]]]]]]]; simplify_eq.
+    elim/lt_wf_ind: m sp ipfs cs K Kl Kr e1' el' er' bl br HK Hm => m IHm.
+    move => ipfs cs sp K Kl Kr e1' el' er' bl br HK Hmatch.
+    case_match; destruct_all?; simplify_eq/=.
+    - destruct (to_val el') eqn:?; [ |apply: Hloop; naive_solver].
+      destruct el'; simplify_eq/=.
+      inversion HK; clear HK; simplify_eq/=.
+      * tstep_i. tstep_s. split!; [econs|] => /=. split!.
+        apply: Hloop. by split!.
+      * tstep_s. split!; [econs|] => /=.
+        tstep_s. right. split!; [econs|] => /=.
+        rewrite !expr_fill_app. apply: IHm; [|done|]; [lia|]. split!. by apply static_expr_expr_fill.
+    - destruct (to_val er') eqn:?; [ |apply: Hloop; naive_solver].
+      destruct er'; simplify_eq/=.
+      inversion HK; clear HK; simplify_eq/=.
+      * tstep_i. tstep_s. split!; [econs|] => /=. split!. apply: Hloop. by split!.
+      * tstep_s. split!; [econs|] => /=.
+        tstep_s. right. split!; [econs|] => /=.
+        rewrite !expr_fill_app. apply: IHm; [|done|]; [lia|]. split!. by apply static_expr_expr_fill.
+    - apply: Hloop; naive_solver.
+  }
+  destruct_all?; simplify_eq/=. case_match; destruct_all?; simplify_eq.
+  - tstep_both. apply: steps_impl_step_end => ?? /prim_step_inv[//|?[?[?[?[??]]]]].
+    simplify_eq. revert select (Is_true (static_expr _)) => /static_expr_expr_fill/=[??]//.
+    rewrite -expr_fill_app.
+    invert_all head_step => //.
+    + tstep_s. eexists None. split!; [done..|] => /=.
+      apply: steps_spec_step_end; [econs; [done|by econs]|].
+      move => /=*; destruct_all?; simplify_eq. tend. split!; [done..|].
+      apply: Hloop. rewrite !expr_fill_app. split!; [done..| ].
+      by apply static_expr_expr_fill.
+    + tstep_s. eexists None. split!; [done..|] => /=.
+      apply: steps_spec_step_end; [econs; [done|by econs]|].
+      move => /=*; destruct_all?; simplify_eq. tend. split!; [done..|].
+      apply: Hloop. rewrite !expr_fill_app. split!; [done..| ].
+      by destruct b; apply static_expr_expr_fill.
+    + tstep_s. eexists None. split!; [done..|] => /=.
+      apply: steps_spec_step_end; [econs; [done|by econs]|].
+      move => /=*; destruct_all?; simplify_eq. tend. split!; [done..|].
+      apply: Hloop. rewrite !expr_fill_app. split!; [done..|].
+      apply static_expr_expr_fill. split!. by apply static_expr_subst.
+    + tstep_s. by split!.
+    + revert select ((_ ∪ _) !! _ = Some _) => /lookup_union_Some_raw[?|[??]].
+      * tstep_s. eexists None. split!; [done..|] => /=.
+        apply: steps_spec_step_end; [econs; [done|by econs]|].
+        move => /=??. destruct_all?; simplify_eq. tend. split!; [done..|].
+        apply: Hloop. rewrite !expr_fill_app. split!; [done..|].
+        apply static_expr_expr_fill. split!. apply static_expr_subst_l; [|done]. apply fd_static.
+      * tstep_s. eexists (Some _). split!; [econs|].
+        { by apply not_elem_of_dom. } { by apply elem_of_dom. } simpl.
+        apply: steps_spec_step_end; [econs; [done|by econs]|].
+        move => /=??. destruct_all?; simplify_eq.
+        tstep_s. left. split!; [done|econs|] => /=. case_bool_decide.
+        2: { tstep_s. naive_solver. }
+        tend. split!; [done..|]. apply: Hloop. split!; [by econs|done..|].
+        apply static_expr_subst_l; [|done]. apply fd_static.
+    + revert select ((_ ∪ _) !! _ = None) => /lookup_union_None[??].
+      tstep_s. eexists (Some _). split!; [apply IPFCallLeftToExt; by apply not_elem_of_dom|] => /=.
+      split!; [done|]. apply: steps_spec_step_end; [econs; [done|by econs]|].
+      move => /=??. destruct_all?; simplify_eq. tend. split!; [done..|].
+      apply: Hloop. split!; [by econs|done..].
+  - tstep_both. apply: steps_impl_step_end => ?? /prim_step_inv[//|?[?[?[?[??]]]]].
+    simplify_eq. revert select (Is_true (static_expr _)) => /static_expr_expr_fill/=[??]//.
+    rewrite -expr_fill_app.
+    invert_all head_step => //.
+    + tstep_s. eexists None. split!; [done..|] => /=.
+      apply: steps_spec_step_end; [econs; [done|by econs]|].
+      move => /=*; destruct_all?; simplify_eq. tend. split!; [done..|].
+      apply: Hloop. rewrite !expr_fill_app. split!; [done..|].
+      by apply static_expr_expr_fill.
+    + tstep_s. eexists None. split!; [done..|] => /=.
+      apply: steps_spec_step_end; [econs; [done|by econs]|].
+      move => /=*; destruct_all?; simplify_eq. tend. split!; [done..|].
+      apply: Hloop. rewrite !expr_fill_app. split!; [done..|].
+      by destruct b; apply static_expr_expr_fill.
+    + tstep_s. eexists None. split!; [done..|] => /=.
+      apply: steps_spec_step_end; [econs; [done|by econs]|].
+      move => /=*; destruct_all?; simplify_eq. tend. split!; [done..|].
+      apply: Hloop. rewrite !expr_fill_app. split!; [done..|].
+      apply static_expr_expr_fill. split!. by apply static_expr_subst.
+    + tstep_s. by split!.
+    + revert select ((_ ∪ _) !! _ = Some _) => /lookup_union_Some_raw[?|[??]].
+      * have ? : fns2 !! f = None by apply: map_disjoint_Some_l.
+        tstep_s. eexists (Some _). split!; [econs|].
+        { by apply elem_of_dom. } { by apply not_elem_of_dom. } simpl.
+        apply: steps_spec_step_end; [econs; [done|by econs]|].
+        move => /=??. destruct_all?; simplify_eq.
+        tstep_s. left. split!; [done|econs|] => /=. case_bool_decide.
+        2: { tstep_s. naive_solver. }
+        tend. split!; [done..|]. apply: Hloop. split!; [by econs|done..|].
+        apply static_expr_subst_l; [|done]. apply fd_static.
+      * tstep_s. eexists None. split!; [done..|] => /=.
+        apply: steps_spec_step_end; [econs; [done|by econs]|].
+        move => /=??. destruct_all?; simplify_eq. tend. split!; [done..|].
+        apply: Hloop. rewrite !expr_fill_app. split!; [done..| ].
+        apply static_expr_expr_fill. split!. apply static_expr_subst_l; [|done]. apply fd_static.
+    + revert select ((_ ∪ _) !! _ = None) => /lookup_union_None[??].
+      tstep_s. eexists (Some _). split!; [apply IPFCallRightToExt; by apply not_elem_of_dom|] => /=.
+      split!; [done|]. apply: steps_spec_step_end; [econs; [done|by econs]|].
+      move => /=??. destruct_all?; simplify_eq. tend. split!; [done..|].
+      apply: Hloop. split!; [by econs|rewrite ?orb_true_r; done..].
+  - tstep_i. split.
+    + move => f fn vs /lookup_union_Some_raw[?|[??]].
+      * have ?: fns2 !! f = None by apply: map_disjoint_Some_l.
+        tstep_s. split!; [econs|]. { by apply elem_of_dom. } { by apply not_elem_of_dom. }
+        simpl. split!; [done|].
+        tstep_s. left. split!; [done|by econs|] => /=. case_bool_decide. 2: { tstep_s. naive_solver. }
+        apply Hloop. split!; [by econs|done..| ].
+        apply static_expr_subst_l; [|done]. apply fd_static.
+      * tstep_s. split!; [apply IPFCallExtToRight|]. { by apply not_elem_of_dom. } { by apply elem_of_dom. }
+        split!; [done|].
+        tstep_s. left. split!; [done|econs|] => /=. case_bool_decide. 2: { tstep_s. naive_solver. }
+        apply Hloop. split!; [by econs|done..| ].
+        apply static_expr_subst_l; [|done]. apply fd_static.
+    + move => v ?.
+      revert select (imp_link_prod_combine_ectx _ _ _ _ _ _ _) => HK.
+      inversion HK; clear HK; simplify_eq/= => //.
+      * tstep_s. split!;[apply IPFReturnExtToLeft|] => /=. split!; [done|].
+        tstep_s. right. split!; [econs|] => /=.
+        apply Hloop. rewrite !expr_fill_app. split!; [done..|].
+        by apply static_expr_expr_fill.
+      * tstep_s. split!; [apply IPFReturnExtToRight|] => /=. split!; [done|].
+        tstep_s. right. split!; [econs|] => /=.
+        apply Hloop. rewrite !expr_fill_app. split!;[done..| ].
+        by apply static_expr_expr_fill.
+Qed.
 
 Lemma imp_prod_refines_link fns1 fns2:
   fns1 ##ₘ fns2 →
